SSAValues.thy
@@ -4,42 +4,21 @@ begin
 
 section "Simps"
 
-lemma memory_\<alpha>_eq[simp]: "memory_\<alpha> (l,s,h) = memory_\<alpha> (l',s,h)"
+lemma memory_\<alpha>_eq[simp]: "memory_\<alpha> (vs,s,h) = memory_\<alpha> (vs',s,h)"
   apply (rule ext)
   subgoal for x
     by (cases x; simp)
   done
 
+lemma ssa_set_\<alpha>_update_eq[simp]:
+  "ssa_set_\<alpha> (ssa (Mapping.update n v m) (insert n a), s, h) = (ssa_set_\<alpha> (ssa m a, s, h))(n := True)"
+  by (auto simp: fun_eq_iff)
 
-lemma ssa_layer_\<alpha>_update_eq_bottom[simp]:
-  "ssa_layer_\<alpha> (ssa_bottom (Mapping.update n v l), s, h) = (ssa_layer_\<alpha> (ssa_bottom l, s, h))(ssa_val n := Some v)"
-  apply (auto simp: fun_eq_iff)
+lemma ssa_\<alpha>_update_eq[simp]:
+  "ssa_\<alpha> (ssa (Mapping.update n v m) (insert n a), s, h) = (ssa_\<alpha> (ssa m a, s, h))(ssa_val n := Some v)"
+  apply (auto simp: fun_eq_iff split: llvm_value_ref.split)
   subgoal for x by (cases x; simp)
   done
-
-lemma ssa_layer_\<alpha>_update_eq_layer[simp]:
-  "ssa_layer_\<alpha> (ssa_layer (Mapping.update n v l) ls, s, h) = (ssa_layer_\<alpha> (ssa_layer l ls, s, h))(ssa_val n := Some v)"
-  apply (auto simp: fun_eq_iff)
-  subgoal for x by (cases x; simp)
-  done
-
-
-lemma ssa_\<alpha>_update_eq_bottom[simp]:
-  "ssa_\<alpha> (ssa_bottom (Mapping.update n v l), s, h) = (ssa_\<alpha> (ssa_bottom l, s, h))(ssa_val n := Some v)"
-  apply (auto simp: fun_eq_iff)
-  subgoal for x by (cases x; simp)
-  done
-
-lemma ssa_\<alpha>_update_eq_layer[simp]:
-  "ssa_\<alpha> (ssa_layer (Mapping.update n v l) ls, s, h) = (ssa_\<alpha> (ssa_layer l ls, s, h))(ssa_val n := Some v)"
-  apply (auto simp: fun_eq_iff)
-  subgoal for x by (cases x; simp)
-  done
-
-
-lemma ssa_layer_\<alpha>_implies_ssa_\<alpha>[simp]:
-  "ssa_layer_\<alpha> (l,s,h) n = Some v \<Longrightarrow> ssa_\<alpha> (l,s,h) n = Some v"
-  by (induction l; cases n; simp)
 
 
 section "Lemmas"
@@ -47,35 +26,34 @@ section "Lemmas"
 named_theorems ssa_value_intro
 
 lemma wp_set_ssa_value_intro[THEN consequence, ssa_value_intro]:
-  assumes "ssa_layer_\<alpha> (l,s,h) (ssa_val n) = None"
-  shows "wp (set_ssa_value l n v) (\<lambda>l'. ssa_layer_\<alpha> (l',s,h) = (ssa_layer_\<alpha> (l,s,h))(ssa_val n := Some v) \<and> ssa_\<alpha> (l',s,h) = (ssa_\<alpha> (l,s,h))(ssa_val n := Some v) \<and> memory_\<alpha> (l',s,h) = memory_\<alpha> (l,s,h))"
+  assumes "\<not>ssa_set_\<alpha> (vs,s,h) n"
+  shows "wp (set_ssa_value vs n v) (\<lambda>vs'. ssa_set_\<alpha> (vs',s,h) = (ssa_set_\<alpha> (vs,s,h))(n := True) \<and> ssa_\<alpha> (vs',s,h) = (ssa_\<alpha> (vs,s,h))(ssa_val n := Some v) \<and> memory_\<alpha> (vs',s,h) = memory_\<alpha> (vs,s,h))"
   using assms
-  by (cases l; simp; intro wp_intro; simp)
+  by (cases vs; simp; intro wp_intro; simp)
 
 lemma wp_set_ssa_intro[THEN consequence, wp_intro]:
-  assumes "ssa_layer_\<alpha> s (ssa_val n) = None"
-  shows "wp (set_ssa s n v) (\<lambda>s'. ssa_layer_\<alpha> s' = (ssa_layer_\<alpha> s)(ssa_val n := Some v) \<and> ssa_\<alpha> s' = (ssa_\<alpha> s)(ssa_val n := Some v) \<and> memory_\<alpha> s' = memory_\<alpha> s)"
+  assumes "\<not>ssa_set_\<alpha> s n"
+  shows "wp (set_ssa s n v) (\<lambda>s'. ssa_set_\<alpha> s' = (ssa_set_\<alpha> s)(n := True) \<and> ssa_\<alpha> s' = (ssa_\<alpha> s)(ssa_val n := Some v) \<and> memory_\<alpha> s' = memory_\<alpha> s)"
   unfolding set_ssa_def
   using assms
   by (intro wp_intro ssa_value_intro wp_return_intro; simp)
 
 
-lemma wp_new_ssa_layer_intro[THEN consequence, wp_intro]:
-  shows "wp (return (new_ssa_layer s)) (\<lambda>s'. ssa_layer_\<alpha> s' = (\<lambda>n. case n of val v \<Rightarrow> Some v | ssa_val _ \<Rightarrow> None) \<and> ssa_\<alpha> s' = ssa_\<alpha> s \<and> memory_\<alpha> s' = memory_\<alpha> s)"
+lemma wp_reset_ssa_assigned_intro[THEN consequence, wp_intro]:
+  shows "wp (return (reset_ssa_assigned s)) (\<lambda>s'. ssa_set_\<alpha> s' = (\<lambda>n. False) \<and> ssa_\<alpha> s' = ssa_\<alpha> s \<and> memory_\<alpha> s' = memory_\<alpha> s)"
   apply (cases s; simp)
-  apply (intro wp_intro wp_return_intro)
-  unfolding new_ssa_value_layer_def
-  apply (auto; rule ext)
-  subgoal for _ _ _ n by (cases n; simp)
-  subgoal for _ _ _ n by (cases n; simp)
+  apply (intro wp_intro wp_return_intro; auto; rule ext)
+  subgoal for vs _ _ n by (cases vs; cases n; simp)
+  subgoal for vs _ _ n by (cases vs; cases n; simp)
+  subgoal for vs _ _ n by (cases vs; cases n; simp)
   done
 
 
 lemma wp_get_ssa_value_intro[THEN consequence, ssa_value_intro]:
-  assumes "ssa_\<alpha> (l,s,h) (ssa_val n) = Some v"
-  shows "wp (get_ssa_value l n) (\<lambda>v'. v' = v)"
+  assumes "ssa_\<alpha> (vs,s,h) (ssa_val n) = Some v"
+  shows "wp (get_ssa_value vs n) (\<lambda>v'. v' = v)"
   using assms
-  by (induction l; simp; intro wp_intro; simp add: option.case_eq_if split: if_splits)
+  by (induction vs; simp; intro wp_intro; simp add: option.case_eq_if split: if_splits)
 
 lemma wp_get_ssa_intro[THEN consequence, wp_intro]:
   assumes "ssa_\<alpha> s n = Some v"
